full embedding of c lang

extract/main.ml
@@ -13,14 +13,14 @@ open ModSemE
 
 (* open MWAll *)
 open Tiny_main
-open Tw_main
+(* open Tw_main *)
 
 let cl2s = fun cl -> String.concat "" (List.map (String.make 1) cl)
 
 module Nat = struct
   include Nat
   let rec to_int = function | O -> 0 | S n -> succ (to_int n)
-  let rec of_int n = assert(n >= 0); if(n == 0) then O else S (of_int (pred n))
+  let rec of_int n = assert(n >= 0); if(n == 0) then O else S (of_int (n - 1))
 end
 
 module Z = struct
@@ -134,5 +134,5 @@ let main =
   (* | 7 -> run (echo_spec_itr) *)
   (* | 8 -> run (sch_exam) *)
   | 9 -> run (Tiny_main.test_itr)
-  | 10 -> run (Tw_main.test_itr)
+  (* | 10 -> run (Tw_main.test_itr) *)
   | _ -> print_endline "Invalid Number!"
